% Penn Bauman
% pcb8gb@virginia.edu
\documentclass[12pt]{article}
\usepackage[utf8]{inputenc}
\usepackage[english]{babel}
\usepackage[top=1in,bottom=1.4in,left=1.25in,right=1.25in,centering,letterpaper]{geometry}
\usepackage{latexsym}
\usepackage[osf]{mathpazo}
\usepackage{amsmath,amsfonts,graphicx}
\usepackage{clrscode}

\author{Penn Bauman}
\title{Answer Distribution Calculations}

\begin{document}

\section{Answer Distribution Calculations}

Basic Requirements:
\begin{align*}
	f(t) &= \lambda e^{-\lambda t} \\
	F(T) &= \int_{0}^{T} f(t) dt \\
	F(\infty) &= 1 \\
	E[f(t)] &= \mu \\
\end{align*}
Determine $F(T)$:
\begin{align*}
	F(T) &= \int_{0}^{T} f(t) dt \\
		&= \int_{0}^{T} \lambda e^{-\lambda t} dt \\
		&= \left[-e^{-\lambda t}\right]_{0}^{T} \\
		&= -e^{-\lambda T} + e^{-\lambda 0} \\
	F(T) &= 1 - e^{-\lambda T}
\end{align*}
Determine $\lambda$:
\begin{align*}
	E[f(t)] &= \int_{0}^{\infty} t f(t) dt \\
		&= \int_{0}^{\infty} \lambda t e^{-\lambda t} dt \\
	u = t & \ \ \ \ \ \ \ \ \ dv = \lambda e^{-\lambda t} dt \\
	du  =  dt & \ \ \ \ \ \ \ \ \ v = -e^{-\lambda t} \\
		&= \left[-t e^{-\lambda t}\right]_{0}^{\infty} - \int_{0}^{\infty} - e^{-\lambda t} dt \\
		&= \left[-t e^{-\lambda t} - \frac{e^{-\lambda t}}{\lambda}\right]_{0}^{\infty} \\
		&= -\infty e^{-\lambda \infty} - \frac{e^{-\lambda \infty}}{\lambda}
		+ 0 e^{-\lambda 0} + \frac{e^{-\lambda 0}}{\lambda} \\
		&= 0 - 0 + 0 + \frac{1}{\lambda} \\
	\mu &= \frac{1}{\lambda} \\
	\lambda &= \frac{1}{\mu} \\
\end{align*}

Forcing time below a maximum:
\begin{align*}
	f(t) &= A \lambda e^{-\lambda t} \\
	F(T) &= \int_{0}^{T} f(t) dt \\
	F(t_{max}) &= 1 \\
	\\
	F(T) &= \int_{0}^{T} f(t) dt \\
		&= \int_{0}^{T} A \lambda e^{-\lambda t} dt \\
		&= \left[-A e^{-\lambda t}\right]_{0}^{T} \\
		&= A\left(-e^{-\lambda T} + e^{-\lambda 0}\right) \\
	F(T) &= A\left(1 - e^{-\lambda T}\right) \\
	\\
	F(t_{max}) &= A\left(1 - e^{-\lambda t_{max}}) \\
	1 &= A\left(1 - e^{-\lambda t_{max}}) \\
	A &= \frac{1}{1 - e^{-\lambda t_{max}}}
\end{align*}

Determine $T(F)$:
\begin{align*}
	%F(T) &= 1 - e^{-\lambda T} \\
	%1 - F &= e^{-\lambda T} \\
	%\ln(1 - F) &= \ln(e^{-\lambda T}) \\
	%-\lambda T &= \ln(1 - F) \\
	%T(F) &= \frac{-\ln(1 - F)}{\lambda} \\
	%
	F(T) &= A\left(1 - e^{-\lambda T}\right) \\
	\frac{F}{A} &= 1 - e^{-\lambda T} \\
	e^{-\lambda T} &= 1 - \frac{F}{A} \\
	\ln\left(e^{-\lambda T}\right) &= \ln\left(1 - \frac{F}{A}\right) \\
	-\lambda T &= \ln\left(1 - \frac{F}{A}\right) \\
	T(F) &= \frac{-1}{\lambda}\ln\left(1 - \frac{F}{A}\right) \\
	%
	%F(1 - e^{-25/12}) &= 1 - e^{\frac{-T}{12}} \\
	%e^{\frac{-T}{12}} &= 1 - F(1 - e^{-25/12}) \\
	%\ln\left(e^{\frac{-T}{12}}\right) &= \ln\left(1 - F(1 - e^{-25/12})\right) \\
	%\frac{-T}{12} &= \ln\left(1 - F(1 - e^{-25/12})\right) \\
	%T(F) &= -12 \ln\left(1 - F(1 - e^{-25/12})\right) \\
\end{align*}

Final Equations:
\begin{align*}
	\mu &= 12 \\
	t_{max} &= 25 \\
	\lambda &= \frac{1}{12} \\
	A &= \frac{1}{1 - e^{-25/12}} \\
	\\
	%f(t) &= \frac{1}{12} e^{\frac{-t}{12}} \\
	f(t) &= A \lambda e^{-\lambda t} \\
	f(t) &= \frac{1}{12 (1 - e^{-25/12})} e^{-t/12} \\
	\\
	F(T) &= A\left(1 - e^{-\lambda T}\right) \\
	F(T) &= \frac{1}{1 - e^{-25/12}}\left(1 - e^{\frac{-T}{12}}\right) \\
	%F(T) &= 1 - e^{-T/12} \\
	\\
	T(F) &= \frac{-1}{\lambda}\ln\left(1 - \frac{F}{A}\right) \\
	T(F) &= -12 \ln\left(1 - F(1 - e^{-25/12})\right) \\
\end{align*}


\end{document}
